feat: simplify nested arith expressions

src/Lean/Meta/Tactic/LinearArith/Simp.lean
@@ -7,6 +7,15 @@ import Lean.Meta.Tactic.LinearArith.Nat
 
 namespace Lean.Meta.Linear
 
+/-- Quick filter simpExpr? -/
+private partial def isSimpExprTarget (e : Expr) : Bool :=
+  let f := e.getAppFn
+  if !f.isConst then
+    false
+  else
+    let n := f.constName!
+    n == ``HAdd.hAdd || n == ``HMul.hMul || n == ``HSub.hSub || n == ``Nat.succ
+
 /-- Quick filter simpCnstr? -/
 private partial def isSimpCnstrTarget (e : Expr) : Bool :=
   let f := e.getAppFn
@@ -21,10 +30,18 @@ private partial def isSimpCnstrTarget (e : Expr) : Bool :=
     else
       false
 
-def simpCnstr? (e : Expr) : MetaM (Option (Expr × Expr)) := do
+private def parentIsTarget (parent? : Option Expr) : Bool :=
+  match parent? with
+  | none => false
+  | some parent => isSimpExprTarget parent || isSimpCnstrTarget parent
+
+def simp? (e : Expr) (parent? : Option Expr) : MetaM (Option (Expr × Expr)) := do
+  -- TODO: add support for `Int` and arbitrary ordered comm rings
   if isSimpCnstrTarget e then
-    -- TODO: add support for `Int` and arbitrary ordered comm rings
     Nat.simpCnstr? e
+  else if isSimpExprTarget e && !parentIsTarget parent? then
+    trace[Meta.Tactic.simp] "arith expr: {e}"
+    Nat.simpExpr? e
   else
     return none
 
